\documentclass{ximera}
\input{../preamble.tex}

\title{Exercises} \license{CC BY-NC-SA 4.0}

\begin{document}

\begin{abstract}
\end{abstract}
\maketitle

\begin{onlineOnly}
\section*{Exercises}
\end{onlineOnly}

\begin{problem}\label{exer:8.7.1}
Solve the initial value
problem.
 $y''+3y'+2y=6e^{2t}+2\delta(t-1), \quad  y(0)=2,\quad y'(0)=-6$
\end{problem}

\begin{problem}\label{exer:8.7.2} 
Solve the initial value
problem.  Graph the solution.
 $y''+y'-2y=-10e^{-t}+5\delta(t-1), \quad  y(0)=7,\quad y'(0)=-9$
\end{problem}

\begin{problem}\label{exer:8.7.3}
Solve the initial value
problem.
 $y''-4y=2e^{-t}+5\delta(t-1), \quad  y(0)=-1,\quad y'(0)=2$
\end{problem}

\begin{problem}\label{exer:8.7.4}  Solve the initial value problem.  Graph the solution.
 $y''+y=\sin3t+2\delta(t-\pi/2), \quad  y(0)=1,\quad y'(0)=-1$
\end{problem}

\begin{problem}\label{exer:8.7.5} 
Solve the initial value
problem.
 $y''+4y=4+\delta(t-3\pi), \quad  y(0)=0,\quad y'(0)=1$
\end{problem}

\begin{problem}\label{exer:8.7.6}
Solve the initial value
problem.
 $y''-y=8+2\delta(t-2), \quad  y(0)=-1,\quad y'(0)=1$
\end{problem}

\begin{problem}\label{exer:8.7.7}
Solve the initial value
problem.
 $y''+y'=e^t+3\delta(t-6), \quad  y(0)=-1,\quad y'(0)=4$
\end{problem}

\begin{problem}\label{exer:8.7.8}
Solve the initial value
problem.
 $y''+4y=8e^{2t}+\delta(t-\pi/2), \quad  y(0)=8,\quad y'(0)=0$
\end{problem}

\begin{problem}\label{exer:8.7.9} Solve the initial value problem.  Graph the solution.
 $y''+3y'+2y=1+\delta(t-1), \quad  y(0)=1,\quad y'(0)=-1$
\end{problem}

\begin{problem}\label{exer:8.7.10}
Solve the initial value
problem.
 $y''+2y'+y=e^t+2\delta(t-2), \quad  y(0)=-1,\quad y'(0)=2$
\end{problem}

\begin{problem}\label{exer:8.7.11} Solve the initial value problem.  Graph the solution.
 $y''+4y=\sin t+\delta(t-\pi/2), \quad  y(0)=0,\quad y'(0)=2$
\end{problem}

\begin{problem}\label{exer:8.7.12}
Solve the initial value
problem.
 $y''+2y'+2y=\delta(t-\pi)-3\delta(t-2\pi), \quad  y(0)=-1,\quad y'(0)=2$
\end{problem}

\begin{problem}\label{exer:8.7.13}
Solve the initial value
problem.
$y''+4y'+13y=\delta(t-\pi/6)+2\delta(t-\pi/3), \quad  y(0)=1,\quad y'(0)=2$
\end{problem}

\begin{problem}\label{exer:8.7.14}
Solve the initial value
problem.
$2y''-3y'-2y=1+\delta(t-2), \quad  y(0)=-1,\quad y'(0)=2$
\end{problem}

\begin{problem}\label{exer:8.7.15}
Solve the initial value
problem.
$4y''-4y'+5y=4\sin t-4\cos
t+\delta(t-\pi/2)-\delta(t-\pi), \quad  y(0)=1,\quad y'(0)=1$
\end{problem}

\begin{problem}\label{exer:8.7.16}
Solve the initial value
problem.
$y''+y=\cos2t+2\delta(t-\pi/2)-3\delta(t-\pi), \quad  y(0)=0,\quad y'(0)=-1$
\end{problem}

\begin{problem}\label{exer:8.7.17} Solve the initial value problem.  Graph the solution.
$y''-y=4e^{-t}-5\delta(t-1)+3\delta(t-2), \quad  y(0)=0,\quad y'(0)=0$
\end{problem}

\begin{problem}\label{exer:8.7.18}
Solve the initial value
problem.
$y''+2y'+y=e^t-\delta(t-1)+2\delta(t-2), \quad  y(0)=0,\quad y'(0)=-1$
\end{problem}

\begin{problem}\label{exer:8.7.19}
Solve the initial value
problem.
$y''+y=f(t)+\delta(t-2\pi), \quad  y(0)=0,\quad y'(0)=1$, \text{and}

$f(t)=\left\{\begin{array}{cl}
\sin2t,&0\le t<\pi,\\0,&t\ge \pi.\end{array}\right.$
\end{problem}

\begin{problem}\label{exer:8.7.20}
Solve the initial value
problem.
$y''+4y=f(t)+\delta(t-\pi)-3\delta(t-3\pi/2), \quad  y(0)=1,\quad
y'(0)=-1$, \text {and}

$f(t)=\left\{\begin{array}{cl}1,&0\le t<\pi/2,\\2,&t\ge
\pi/2\end{array}\right.$
\end{problem}

\begin{problem}\label{exer:8.7.21}
Solve the initial value
problem.
$y''+y=\delta(t), \quad  y(0)=1,\quad y_-'(0)=-2$
\end{problem}

\begin{problem}\label{exer:8.7.22}
Solve the initial value
problem.
$y''-4y=3\delta(t), \quad  y(0)=-1,\quad y_-'(0)=7$
\end{problem}

\begin{problem}\label{exer:8.7.23}
Solve the initial value
problem.
$y''+3y'+2y=-5\delta(t), \quad  y(0)=0,\quad y_-'(0)=0$
\end{problem}

\begin{problem}\label{exer:8.7.24}
Solve the initial value
problem.
$y''+4y'+4y=-\delta(t), \quad  y(0)=1,\quad y_-'(0)=5$
\end{problem}

\begin{problem}\label{exer:8.7.25}
Solve the initial value
problem.
$4y''+4y'+y=3\delta(t), \quad  y(0)=1,\quad y_-'(0)=-6$
\end{problem}

\begin{problem}\label{exer:8.7.26} Solve the initial value problem
$$
ay_h''+by_h'+cy_h=
\left\{\begin{array}{cl} 0,&0\le t<t_0,\\
1/h,&t_0\le t< t_0+h,\\
0,&t\ge t_0+h,\end{array}\right.
\quad y_h(0)=0,\quad y_h'(0)=0,
$$
where $t_0>0$ and $h>0$. Then find
$$
w={\cal L}^{-1}\left(\frac{1}{as^2+bs+c}\right)
$$
and verify Theorem~\ref{thmtype:8.7.1} by graphing $w$ and $y_h$
on the same axes, for small positive values of $h$.
$y''+2y'+2y=f_h(t), \quad  y(0)=0,\quad y'(0)=0$
\end{problem}

\begin{problem}\label{exer:8.7.27} Solve the initial value problem
$$
ay_h''+by_h'+cy_h=
\left\{\begin{array}{cl} 0,&0\le t<t_0,\\
1/h,&t_0\le t< t_0+h,\\
0,&t\ge t_0+h,\end{array}\right.
\quad y_h(0)=0,\quad y_h'(0)=0,
$$
where $t_0>0$ and $h>0$. Then find
$$
w={\cal L}^{-1}\left(\frac{1}{as^2+bs+c}\right)
$$
and verify Theorem~\ref{thmtype:8.7.1} by graphing $w$ and $y_h$
on the same axes, for small positive values of $h$.
$y''+2y'+y=f_h(t), \quad  y(0)=0,\quad y'(0)=0$
\end{problem}

\begin{problem}\label{exer:8.7.28} Solve the initial value problem
$$
ay_h''+by_h'+cy_h=
\left\{\begin{array}{cl} 0,&0\le t<t_0,\\
1/h,&t_0\le t< t_0+h,\\
0,&t\ge t_0+h,\end{array}\right.
\quad y_h(0)=0,\quad y_h'(0)=0,
$$
where $t_0>0$ and $h>0$. Then find
$$
w={\cal L}^{-1}\left(\frac{1}{as^2+bs+c}\right)
$$
and verify Theorem~\ref{thmtype:8.7.1} by graphing $w$ and $y_h$
on the same axes, for small positive values of $h$.
$y''+3y'+2y=f_h(t), \quad  y(0)=0,\quad y'(0)=0$
\end{problem}

\begin{problem}\label{exer:8.7.29}

Recall from Section~6.2 that the displacement of
an
object of mass $m$ in a spring--mass system in free damped oscillation is
$$
my''+cy'+ky=0, \quad  y(0)=y_0,\quad y'(0)=v_0,
$$
and that $y$ can be written as
$$
y=Re^{-ct/2m}\cos(\omega_1t-\phi)
$$
if the motion is underdamped. Suppose $y(\tau)=0$.
Find the impulse that would have to be applied to the object at $t=\tau$
 to put it in equilibrium.
\end{problem}

\begin{problem}\label{exer:8.7.30}
\begin{enumerate}

\item Solve the initial value problem. Find a formula that
does not involve step functions and represents $y$  on each subinterval of $[0,\infty)$ on which the forcing function is zero.
$y''-y=\sum_{k=1}^\infty\delta(t-k), \quad  y(0)=0,\quad y'(0)=1$

\item Solve the initial value problem. Find a formula that
does not involve step functions and represents $y$  on each subinterval of $[0,\infty)$ on which the forcing function is zero.
$y''+y=\sum_{k=1}^\infty\delta(t-2k\pi), \quad  y(0)=0,\quad y'(0)=1$

\item Solve the initial value problem. Find a formula that
does not involve step functions and represents $y$  on each subinterval of $[0,\infty)$ on which the forcing function is zero.
$y''-3y'+2y=\sum_{k=1}^\infty\delta(t-k), \quad  y(0)=0,\quad y'(0)=1$

\item Solve the initial value problem. Find a formula that
does not involve step functions and represents $y$  on each subinterval of $[0,\infty)$ on which the forcing function is zero.
$y''+y=\sum_{k=1}^\infty\delta(t-k\pi), \quad  y(0)=0,\quad y'(0)=0$
\end{enumerate}
\end{problem}

\end{document}