\documentclass{ximera}
\input{../preamble.tex}

\title{Exercises} \license{CC BY-NC-SA 4.0}

\begin{document}

\begin{abstract}
\end{abstract}
\maketitle

\begin{onlineOnly}
\section*{Exercises}
\end{onlineOnly}


\begin{problem}\label{exer:5.6.1}
Find the general solution,
given that $y_1$ satisfies the complementary equation. As a by-product,
find a fundamental set of solutions of the complementary equation. $(2x+1)y''-2y'-(2x+3)y=(2x+1)^2;  \quad y_1=e^{-x}$
\end{problem}

\begin{problem}\label{exer:5.6.2}
Find the general solution,
given that $y_1$ satisfies the complementary equation. As a by-product,
find a fundamental set of solutions of the complementary equation. $x^2y''+xy'-y=\frac{4}{x^2};   \quad y_1=x$
\end{problem}

\begin{problem}\label{exer:5.6.3}
Find the general solution,
given that $y_1$ satisfies the complementary equation. As a by-product,
find a fundamental set of solutions of the complementary equation. $x^2y''-xy'+y=x;   \quad y_1=x$
\end{problem}

\begin{problem}\label{exer:5.6.4}
Find the general solution,
given that $y_1$ satisfies the complementary equation. As a by-product,
find a fundamental set of solutions of the complementary equation. $y''-3y'+2y=\frac{1}{1+e^{-x}};   \quad y_1=e^{2x}$
\end{problem}

\begin{problem}\label{exer:5.6.5}
Find the general solution,
given that $y_1$ satisfies the complementary equation. As a by-product,
find a fundamental set of solutions of the complementary equation. $y''-2y'+y=7x^{3/2}e^x;   \quad y_1=e^x$
\end{problem}

\begin{problem}\label{exer:5.6.6}
Find the general solution,
given that $y_1$ satisfies the complementary equation. As a by-product,
find a fundamental set of solutions of the complementary equation. $4x^2y''+(4x-8x^2)y'+(4x^2-4x-1)y=4x^{1/2}e^x(1+4x);   \quad
y_1=x^{1/2}e^x$
\end{problem}

\begin{problem}\label{exer:5.6.7}
Find the general solution,
given that $y_1$ satisfies the complementary equation. As a by-product,
find a fundamental set of solutions of the complementary equation. $y''-2y'+2y=e^x\sec x;   \quad y_1=e^x\cos x$
\end{problem}

\begin{problem}\label{exer:5.6.8}
Find the general solution,
given that $y_1$ satisfies the complementary equation. As a by-product,
find a fundamental set of solutions of the complementary equation. $y''+4xy'+(4x^2+2)y=8e^{-x(x+2)};   \quad y_1=e^{-x^2}$
\end{problem}

\begin{problem}\label{exer:5.6.9}
Find the general solution,
given that $y_1$ satisfies the complementary equation. As a by-product,
find a fundamental set of solutions of the complementary equation. $x^2y''+xy'-4y=-6x-4;  \quad y_1=x^2$
\end{problem}

\begin{problem}\label{exer:5.6.10}
Find the general solution,
given that $y_1$ satisfies the complementary equation. As a by-product,
find a fundamental set of solutions of the complementary equation. $x^2y''+2x(x-1)y'+(x^2-2x+2)y=x^3e^{2x};   \quad y_1=xe^{-x}$
\end{problem}

\begin{problem}\label{exer:5.6.11}
Find the general solution,
given that $y_1$ satisfies the complementary equation. As a by-product,
find a fundamental set of solutions of the complementary equation. $x^2y''-x(2x-1)y'+(x^2-x-1)y=x^2e^x;  \quad y_1=xe^x$
\end{problem}

\begin{problem}\label{exer:5.6.12}
Find the general solution,
given that $y_1$ satisfies the complementary equation. As a by-product,
find a fundamental set of solutions of the complementary equation. $(1-2x)y''+2y'+(2x-3)y=(1-4x+4x^2)e^x;  \quad y_1=e^x$
\end{problem}

\begin{problem}\label{exer:5.6.13}
Find the general solution,
given that $y_1$ satisfies the complementary equation. As a by-product,
find a fundamental set of solutions of the complementary equation. $x^2y''-3xy'+4y=4x^4;  \quad y_1=x^2$
\end{problem}

\begin{problem}\label{exer:5.6.14}
Find the general solution,
given that $y_1$ satisfies the complementary equation. As a by-product,
find a fundamental set of solutions of the complementary equation. $2xy''+(4x+1)y'+(2x+1)y=3x^{1/2}e^{-x};  \quad y_1=e^{-x}$
\end{problem}

\begin{problem}\label{exer:5.6.15}
Find the general solution,
given that $y_1$ satisfies the complementary equation. As a by-product,
find a fundamental set of solutions of the complementary equation. $xy''-(2x+1)y'+(x+1)y=-e^x;  \quad y_1=e^x$
\end{problem}

\begin{problem}\label{exer:5.6.16}
Find the general solution,
given that $y_1$ satisfies the complementary equation. As a by-product,
find a fundamental set of solutions of the complementary equation. $4x^2y''-4x(x+1)y'+(2x+3)y=4x^{5/2}e^{2x};  \quad y_1=x^{1/2}$
\end{problem}

\begin{problem}\label{exer:5.6.17}
Find the general solution,
given that $y_1$ satisfies the complementary equation. As a by-product,
find a fundamental set of solutions of the complementary equation. $x^2y''-5xy'+8y=4x^2;  \quad y_1=x^2$
\end{problem}

\begin{problem}\label{exer:5.6.18} Find a
fundamental set of solutions, given that $y_1$ is a solution. $xy''+(2-2x)y'+(x-2)y=0;    \quad y_1=e^x$
\end{problem}

\begin{problem}\label{exer:5.6.19}
Find a
fundamental set of solutions, given that $y_1$ is a solution. $x^2y''-4xy'+6y=0;   \quad y_1=x^2$
\end{problem}

\begin{problem}\label{exer:5.6.20}
Find a
fundamental set of solutions, given that $y_1$ is a solution. $x^2(\ln |x|)^2y''-(2x \ln |x|)y'+(2+\ln |x|)y=0;   \quad y_1=\ln |x|$
\end{problem}

\begin{problem}\label{exer:5.6.21}
Find a
fundamental set of solutions, given that $y_1$ is a solution. $4xy''+2y'+y=0;  \quad y_1=\sin \sqrt{x}$
\end{problem}

\begin{problem}\label{exer:5.6.22}
Find a
fundamental set of solutions, given that $y_1$ is a solution. $xy''-(2x+2)y'+(x+2)y=0;   \quad y_1=e^x$
\end{problem}

\begin{problem}\label{exer:5.6.23}
Find a
fundamental set of solutions, given that $y_1$ is a solution. $x^2y''-(2a-1)xy'+a^2y=0;   \quad y_1=x^a$
\end{problem}

\begin{problem}\label{exer:5.6.24}
Find a
fundamental set of solutions, given that $y_1$ is a solution. $x^2y''-2xy'+(x^2+2)y=0;   \quad y_1=x \sin x$
\end{problem}

\begin{problem}\label{exer:5.6.25}
Find a
fundamental set of solutions, given that $y_1$ is a solution. $xy''-(4x+1)y'+(4x+2)y=0;  \quad y_1=e^{2x}$
\end{problem}

\begin{problem}\label{exer:5.6.26}
Find a
fundamental set of solutions, given that $y_1$ is a solution. $4x^2(\sin x)y''-4x(x\cos x+\sin x)y'+(2x\cos x+3\sin x)y=0;  \quad
y_1=x^{1/2}$
\end{problem}

\begin{problem}\label{exer:5.6.27}
Find a
fundamental set of solutions, given that $y_1$ is a solution. $4x^2y''-4xy'+(3-16x^2)y=0;  \quad y_1=x^{1/2}e^{2x}$
\end{problem}

\begin{problem}\label{exer:5.6.28}
Find a
fundamental set of solutions, given that $y_1$ is a solution. $(2x+1)xy''-2(2x^2-1)y'-4(x+1)y=0;  \quad y_1=1/x$
\end{problem}

\begin{problem}\label{exer:5.6.29}
Find a
fundamental set of solutions, given that $y_1$ is a solution. $(x^2-2x)y''+(2-x^2)y'+(2x-2)y=0;  \quad y_1=e^x$
\end{problem}

\begin{problem}\label{exer:5.6.30}
Find a
fundamental set of solutions, given that $y_1$ is a solution. $xy''-(4x+1)y'+(4x+2)y=0;  \quad y_1=e^{2x}$
\end{problem}

\begin{problem}\label{exer:5.6.31}
Solve the
initial value problem, given that $y_1$ satisfies the complementary
equation. $x^2y''-3xy'+4y=4x^4,\quad y(-1)=7,\quad  y'(-1)=-8;   \quad y_1=x^2$
\end{problem}

\begin{problem}\label{exer:5.6.32}
Solve the
initial value problem, given that $y_1$ satisfies the complementary
equation. $(3x-1)y''-(3x+2)y'-(6x-8)y=0, \quad   y(0)=2,\;  y'(0)=3;    \quad
y_1=e^{2x}$
\end{problem}

\begin{problem}\label{exer:5.6.33}
Solve the
initial value problem, given that $y_1$ satisfies the complementary
equation. $(x+1)^2y''-2(x+1)y'-(x^2+2x-1)y=(x+1)^3e^x, \quad  y(0)=1,\quad y'(0)=~-1$;

$y_1=(x+1)e^x$
\end{problem}

\begin{problem}\label{exer:5.6.34} Solve the
initial value problem and graph the solution, given that $y_1$
satisfies the complementary equation.
$x^2y''+2xy'-2y=x^2, \quad   y(1)=\frac{5}{4},\;
y'(1)=\frac{3}{2};   \quad y_1=x$
\end{problem}

\begin{problem}\label{exer:5.6.35} Solve the
initial value problem and graph the solution, given that $y_1$
satisfies the complementary equation.
$(x^2-4)y''+4xy'+2y=x+2, \quad  y(0)=-\frac{1}{3},\quad y'(0)=-1;
\quad y_1=\frac{1}{x-2}$
\end{problem}

\begin{problem}\label{exer:5.6.36}
Suppose $p_1$ and $p_2$ are continuous on $(a,b)$. Let $y_1$
be a solution of
\begin{equation}\label{eq:eqA5.6.36}
 y''+p_1(x)y'+p_2(x)y=0
\end{equation}
that has no zeros on $(a,b)$, and let $x_0$ be in $(a,b)$.
Use reduction of order to show that $y_1$ and
$$
y_2(x)=y_1(x)\int^x_{x_0}\frac{1}{y^2_1(t)} \exp
\left(-\int^t_{x_0}p_1(s)\, ds\right)\,dt
$$
form a fundamental set of solutions of \ref{eq:eqA5.6.36} on
$(a,b)$.
(This exercise is related to Exercise~\ref{exer:5.1.9}.)
\end{problem}

\begin{problem}\label{exer:5.6.37}
The nonlinear first order equation
\begin{equation}\label{eq:eqA5.6.37}
y'+y^2+p(x)y+q(x)=0
\end{equation}
is a
\href{http://http://www-history.mcs.st-and.ac.uk/Indexes/Riccati.html}
{Riccati equation}.  (See
Exercise~\ref{exer:2.4.55}.) Assume that $p$ and $q$ are continuous.
\begin{enumerate}
\item %(a)
Show that $y$ is a solution of \ref{eq:eqA5.6.37} if and only if $y={z'/z}$, where
\begin{equation}\label{eq:eqB5.6.37}
z''+p(x)z'+q(x)z=0.
\end{equation}

\item %(b)
 Show that the general solution of \ref{eq:eqA5.6.37} is
\begin{equation}\label{eq:eqC5.6.37}
y=\frac{c_1z'_1+c_2z'_2}{c_1z_1+c_2z_2},
\end{equation}
where $\{z_1,z_2\}$ is a fundamental
set of solutions of \ref{eq:eqB5.6.37} and $c_1$ and $c_2$ are
arbitrary constants.

\item %(c)
Does the formula \ref{eq:eqC5.6.37} imply that the first order equation
\ref{eq:eqA5.6.37} has a two--parameter family of solutions?
Explain your answer.
\end{enumerate}
\end{problem}

\begin{problem}\label{exer:5.6.38}
Use a method suggested by Exercise~\ref{exer:5.6.37}  to find all
solutions of the equation.

\begin{enumerate}

\item $y'+y^2+k^2=0$

\item$y'+y^2-3y+2=0$

\item $y'+y^2+5y-6=0$

\item $y'+y^2+8y+7=0$

\item $y'+y^2+14y+50=0$

\item $6y'+6y^2-y-1=0$


\item $36y'+36y^2-12y+1=0$
\end{enumerate}
\end{problem}

\begin{problem}\label{exer:5.6.39}
Use a method suggested by Exercise~\ref{exer:5.6.37} and reduction of
order to find all solutions of the equation, given that $y_1$ is
a solution.

\begin{enumerate}
\item %(a)
$x^2(y'+y^2)-x(x+2)y+x+2=0;  \quad y_1=1/x$

\item %(b)
$y'+y^2+4xy+4x^2+2=0;   \quad y_1=-2x$

\item %(c)
$(2x+1)(y'+y^2)-2y-(2x+3)=0;   \quad y_1=-1$

\item %(d)
$(3x-1)(y'+y^2)-(3x+2)y-6x+8=0;   \quad y_1=2$

\item %(e)
$x^2(y'+y^2)+xy+x^2-\frac{1}{4}=0;
\quad y_1=-\tan x -\frac{1}{2x}$

\item %(f)
$x^2(y'+y^2)-7xy+7=0;  \quad y_1=1/x$

\end{enumerate}
\end{problem}

\begin{problem}\label{exer:5.6.40}
The nonlinear first order equation
\begin{equation}\label{eq:eqA5.6.40}
 y'+r(x)y^2+p(x)y+q(x)=0
\end{equation}
is the
\href{http://http://www-history.mcs.st-and.ac.uk/Indexes/Riccati.html}
{generalized Riccati equation}.
(See Exercise~\ref{exer:2.4.55}.)
Assume that $p$ and $q$ are continuous and $r$ is differentiable.

\begin{enumerate}
\item %(a)
Show that $y$ is a solution of \ref{eq:eqA5.6.40} if and only if
 $y={z'/rz}$,  where \begin{equation}\label{eq:eqB5.6.40}
z''+\left[p(x)-\frac{r'(x)}{r(x)}\right]
z'+r(x)q(x)z=0.
\end{equation}

\item %(b)
 Show that the general solution of \ref{eq:eqA5.6.40} is
$$
 y=\frac{c_1z'_1+c_2z'_2}{r(c_1z_1+c_2z_2)},
$$
where $\{z_1,z_2\}$ is a fundamental set of solutions of
\ref{eq:eqB5.6.40} and $c_1$ and $c_2$ are arbitrary constants.
\end{enumerate}
\end{problem}

\end{document}