\documentclass{ximera}
\input{../preamble.tex}

\title{Exercises} \license{CC BY-NC-SA 4.0}

\begin{document}

\begin{abstract}
\end{abstract}
\maketitle

\begin{onlineOnly}
\section*{Exercises}
\end{onlineOnly}

\begin{problem}\label{exer:8.5.1} 
Use the Laplace transform to solve the initial value problem.
$y''+y = \left\{\begin{array}{cl} 3,& 0\le t<\pi,\\ 0,&t\ge\pi,\end{array}\right.\qquad y(0)=0, \quad  y'(0)=0$
\end{problem}

\begin{problem}\label{exer:8.5.2} 
Use the Laplace transform to solve the initial value problem.
$y''+y=\left\{\begin{array}{cl} 3,&0\le
t<4,\\ 2t-5,&t > 4,\end{array}\right.\qquad y(0)=1,\quad y'(0)=0$

\begin{solution}
 $y''+y=3+u(t-4)(2t-8),\ y(0)=1,\ y'(0)=0$.
Since
$$
{\cal L}\left(u(t-4)(2t-8)\right)=e^{-4s}{\cal L}\left(2(t+4)-8\right)
=e^{-4s}{\cal L}(2t)=\frac{2e^{-4s}}{s^2},
$$
$$
(s^2+1)Y(s)=\frac{3}{s}+\frac{2e^{-4s}}{s^2}+s.
$$
\begin{eqnarray*}
Y(s)&=&\frac{3}{s(s^2+1)}+\frac{2e^{-4s}}{s^2(s^2+1)}+\frac{s}{s^2+1}\\
&=&3\left(\frac{1}{s}-\frac{s}{s^2+1}\right)+2e^{-4s}
\left(\frac{1}{s^2}-\frac{1}{s^2+1}\right)+\frac{s}{s^2+1}\\
&=&\frac{3}{s}-\frac{2s}{s^2+1}+2e^{-4s}\left(\frac{1}{s^2}-\frac{1}{s^2+1}\right).
\end{eqnarray*}
Since
$$
\frac{1}{s^2}-\frac{1}{s^2+1}\leftrightarrow t-\sin t\Rightarrow
e^{-4s}\left(\frac{1}{s^2}-\frac{1}{s^2+1}\right)\leftrightarrow
u(t-4)\left(t-4-\sin(t-4)\right),
$$
$y=3-2\cos t+2u(t-4)\left(t-4-\sin(t-4)\right)$.
\end{solution}
\end{problem}

\begin{problem}\label{exer:8.5.3} Use the Laplace transform to solve the initial value problem.
$y''-2y'= \left\{\begin{array}{cl} 4,&0\le
t<1,\\ 6,&t\ge 1,\end{array}\right.\qquad y(0)=-6,\quad y'(0)=1$
\end{problem}

\begin{problem}\label{exer:8.5.4} Use the Laplace transform to solve the initial value problem.
$y''-y=\left\{\begin{array}{cl} e^{2t},&0\le
t< 2,\\ 1,&t\ge 2,\end{array}\right.\qquad y(0)=3,\quad y'(0)=-1$
\end{problem}

\begin{problem}\label{exer:8.5.5} Use the Laplace transform to solve the initial value problem.
$y''-3y'+2y= \left\{\begin{array}{rl} 0,&0\le
t<1,\\ 1,&1\le t<2,\\ -1,&t\ge 2,\end{array}\right.\qquad y(0)=-3,\quad y'(0)=1$
\end{problem}

\begin{problem}\label{exer:8.5.6} Use the Laplace transform to solve the initial value problem.  Graph the solution. 
$y''+4y= \left\{\begin{array}{cl}|\sin
t|,&0\le t<2\pi,\\ 0,&t\ge 2\pi,\end{array}\right.\qquad
y(0)=-3,\quad y'(0)=1$

\begin{solution}
Note that $|\sin t|=\sin t$ if $0\le t<\pi$, while
 $|\sin t|=-\sin t$ if $\pi\le t<2\pi$. Rewrite the initial value
problem as
$$
y''+4y=\sin t-2u(t-\pi)\sin t+u(t-2\pi)\sin t,\ y(0)=-3,\ y'(0)=1.
$$
Since
$$
{\cal L}\left(u(t-\pi)\sin t\right)=e^{-\pi s}{\cal
L}(\sin(t+\pi))=-e^{-\pi s}{\cal L}(\sin t)
$$
 and
$$
{\cal L}\left(u(t-2\pi)\sin t\right)=e^{-2\pi s}{\cal
L}(\sin(t+2\pi))=e^{-2\pi s}{\cal L}(\sin t),
$$
$$
(s^2+4)Y(s)=\frac{1+2e^{-\pi s}+e^{-2\pi s}}{(s^2+1)}+1-3s,\mbox{ so }
Y(s)=\frac{1+2e^{-\pi s}+e^{-2\pi
s}}{(s^2+1)(s^2+4)}+\frac{1-3s}{s^2+4}.
$$
$$
\frac{1}{(s^2+1)(s^2+4)}=\left(\frac{1}{s^2+1}-\frac{1}{s^2+4}\right)
\leftrightarrow \frac{1}{3}\sin t-\frac{1}{6}\sin2t;
$$
therefore
\begin{eqnarray*}
\frac{e^{-\pi s}}{(s^2+1)(s^2+4)}
&\leftrightarrow&
u(t-\pi)\left(\frac{1}{3}\sin(t-\pi)-\frac{1}{6}\sin2(t-\pi)\right)\\
&=&-u(t-\pi)\left(\frac{1}{3}\sin t+\frac{1}{6}\sin2t\right)
\end{eqnarray*}
and
\begin{eqnarray*}
\frac{e^{-2\pi s}}{(s^2+1)(s^2+4)}
&\leftrightarrow&
u(t-2\pi)\left(\frac{1}{3}\sin(t-2\pi)-\frac{1}{6}\sin2(t-2\pi)\right)\\
&=&u(t-2\pi)\left(\frac{1}{3}\sin t-\frac{1}{6}\sin2t\right);
\end{eqnarray*}
therefore
$$
y=\frac{1}{3}\sin2t-3\cos2t+\frac{1}{3}\sin t
- 2 u(t-\pi)\left(\frac{1}{3}\sin t+\frac{1}{6}\sin2t\right)
+u(t-2\pi)\left(\frac{1}{3}\sin
t-\frac{1}{6}\sin2t\right).
$$
\end{solution}
\end{problem}

\begin{problem}\label{exer:8.5.7} $y''-5y'+4y= \left\{\begin{array}{rl} 1,&0\le
t<1\\ -1,&1\le t<2,\\ 0,&t\ge 2,\end{array}\right.\qquad
y(0)=3,\quad y'(0)=-5$
\end{problem}

\begin{problem}\label{exer:8.5.8} $y''+9y= \left\{\begin{array}{cl} \cos
t,&0\le t<\frac{3\pi}{2},\\ \sin
t,&t\ge\frac{3\pi}{2},\end{array}\right.\qquad y(0)=0,\;  y'(0)=0$
\end{problem}

\begin{problem}\label{exer:8.5.9} Use the Laplace transform to solve the initial value problem.  Graph the solution. 
$y''+4y= \left\{\begin{array}{cl} t,&0\le
t<\frac{\pi}{2},\\ \pi,&t\ge\frac{\pi}{2},
\end{array}\right.\quad y(0)=0,\quad y'(0)=0$
\end{problem}

\begin{problem}\label{exer:8.5.10}
Use the Laplace transform to solve the initial value problem.
$y''+y=\left\{\begin{array}{cl}-t,&0\le t<\pi,
\\ -t,&t\ge\pi ,\end{array}\right.\;  y(0)=0,\;  y'(0)=0$
\end{problem}

\begin{problem}\label{exer:8.5.11} Use the Laplace transform to solve the initial value problem.
$y''-3y'+2y=\left\{\begin{array}{cl} 0,&0\le
t<2,\\2t-4,&t\ge 2,\end{array}\right. ,\quad y(0)=0,\quad y'(0)=0$

\begin{solution}
$y''+y=t-2u(t-\pi)t,\ y(0)=0,\ y'(0)=0$.
Since
$$
{\cal L}\left(u(t-\pi)t\right)=e^{-\pi s}{\cal L}\left(t+\pi\right)
=e^{-\pi s}\left(\frac{1}{s^2}+\frac{\pi}{s}\right),
$$
$$
(s^2+1)Y(s)=\frac{1}{s^2}-2e^{-\pi s}\left(\frac{1}{s^2}+\frac{\pi}{s}\right);
$$
\begin{eqnarray*}
Y(s)&=& \frac{1}{s^2(s^2+1)}-2e^{-\pi s}\left(\frac{1}{s^2(s^2+1)}+\frac{\pi}{s(s^2+1)}\right)\\ &=&\left(\frac{1}{s^2}-\frac{1}{s^2+1}\right)-2e^{-\pi s} \left(\frac{1}{s^2}-\frac{1}{s^2+1}\right)-2\pi e^{-\pi s}\left(\frac{1}{s}-\frac{s}{s^2+1}\right).
\end{eqnarray*}
Since
\begin{eqnarray*}
\frac{1}{s^2}-\frac{1}{s^2+1}&\leftrightarrow& t-\sin t\Rightarrow
e^{-\pi s}\left(\frac{1}{s^2}-\frac{1}{s^2+1}\right)\\ &\leftrightarrow&
u(t-\pi)\left(t-\pi-\sin(t-\pi)\right)=u(t-\pi)(t-\pi+\sin t)
\end{eqnarray*}
and
\begin{eqnarray*}
\frac{1}{s}-\frac{s}{s^2+1}&\leftrightarrow& 1-\cos t\Rightarrow
e^{-\pi s}\left(\frac{1}{s}-\frac{s}{s^2+1}\right)\\ &\leftrightarrow&
u(t-\pi)\left(1-\cos(t-\pi)\right)=u(t-\pi)(1+\cos t),
\end{eqnarray*}
 $y=t-\sin t-2u(t-\pi)(t+\sin t+\pi\cos t)$.
\end{solution}
\end{problem}

\begin{problem}\label{exer:8.5.12} Use the Laplace transform to solve the initial value problem.
$y''+y=\left\{\begin{array}{cl} t,&0\le
t<2\pi,\\-2t,&t\ge 2\pi,\end{array}\right.\quad y(0)=1,\quad y'(0)=2$
\end{problem}

\begin{problem}\label{exer:8.5.13} Use the Laplace transform to solve the initial value problem.  Graph the solution.
$y''+3y'+2y=\left\{\begin{array}{cl}-1,&0\le
t<2,\\-1,&t\ge 2,\end{array}\right.\;  y(0)=0,\;  y'(0)=0$
\end{problem}

\begin{problem}\label{exer:8.5.14} Use the Laplace transform to solve the initial value problem.
$y''-4y'+3y=\left\{\begin{array}{cl}-1,&0\le
t<1,\\-1,&t\ge 1,\end{array}\right.\;  y(0)=0,\;  y'(0)=0$

\begin{solution}
$y''-4y'+3y=-1+2u(t-1),\ y(0)=0,\ y'(0)=0$;

$(s^2-4s+3)Y(s)=\frac{-1+2e^{-s}}{s}$;
$Y(s)=\frac{-1+2e^{-s}}{s(s-1)(s-3)}$;

$\frac{1}{s(s-1)(s-3)}=\frac{1}{3s}+\frac{1}{6}\frac{1}{s-3}-\frac{1}{2}\frac{1}{s-1}
\leftrightarrow \frac{1}{3}+\frac{1}{6}e^{3t}-\frac{1}{2}e^t$;

$\frac{e^{-s}}{s(s-1)(s-3)}
\leftrightarrow u(t-1)\left(
\frac{1}{3}+\frac{1}{6}e^{3(t-1)}-\frac{1}{2}e^{t-1}\right)$;

$y=-\frac{1}{3}-\frac{1}{6}e^{3t}
+\frac{1}{2}e^t+u(t-1)\left(\frac{2}{3}+\frac{1}{3}e^{3(t-1)}
-e^{t-1}\right)$.
\end{solution}
\end{problem}

\begin{problem}\label{exer:8.5.15} Use the Laplace transform to solve the initial value problem.
$y''+2y'+y=\left\{\begin{array}{cl}
e^t,&0\le t<1,\\e^t-1,&t\ge 1,\end{array}\right.\;  y(0)=3,\;
y'(0)=-1$
\end{problem}

\begin{problem}\label{exer:8.5.16}
Use the Laplace transform to solve the initial value problem.
$y''+2y'+y=\left\{\begin{array}{cl}
4e^t,&0\le t<1,\\0,&t\ge 1,\end{array}\right.\;  y(0)=0,\;
y'(0)=0$
\end{problem}

\begin{problem}\label{exer:8.5.17} Use the Laplace transform to solve the initial value problem.
$y''+3y'+2y=\left\{\begin{array}{cl}
e^{-t},&0\le t<1,\\0,&t\ge 1,\end{array}\right.\;  y(0)=1,\;  y'(0)=-1$
\end{problem}

\begin{problem}\label{exer:8.5.18} Use the Laplace transform to solve the initial value problem.
$y''-4y'+4y=\left\{\begin{array}{rl}
e^{2t},&0\le t<2,\\-e^{2t},&t\ge 2,\end{array}\right.\;  y(0)=0,\;
y'(0)=-1$

\begin{solution}
$y''-4y'+4y=e^{2t}-2u(t-2)e^{2t},\ y(0)=0,\ y'(0)=-1$.
Since
$$
{\cal L}\left(u(t-2)e^{2t}\right)=e^{-2s}{\cal
L}\left(e^{2t+4}\right)=\frac{e^{-2s+4}}{s-2},
$$
$$
(s^2-4s+4)Y(s)=\frac{1}{s-2}-\frac{2e^{-2s+4}}{s-2}-1,\quad\mbox{so}
$$
$$
Y(s)=\frac{1}{(s-2)^3}-\frac{2e^{-2s+4}}{(s-2)^3}-\frac{1}{(s-2)^2}.
$$
$$
\frac{1}{(s-2)^3}\leftrightarrow \frac{t^2e^{2t}}{2}\Rightarrow
\frac{e^{-2s+4}}{(s-2)^3}\leftrightarrow\frac{e^4}{2}u(t-2)e^{2(t-2)}(t-2)^2
=u(t-2)\frac{(t-2)^2e^{2t}}{2};
$$
therefore
$y=\frac{t^2e^{2t}}{2}-te^{2t}-u(t-2)(t-2)^2e^{2t}$.
\end{solution}
\end{problem}

\begin{problem}\label{exer:8.5.19} Use the Laplace transform to solve the initial value problem.  Graph the solution. 
$y''=\left\{\begin{array}{cl}t^2,&0\le
t<1,\\-t,&1\le t<2,\\t+1,&t\ge 2,\end{array}\right.\;  y(0)=1,\;
y'(0)=0$
\end{problem}

\begin{problem}\label{exer:8.5.20} Use the Laplace transform to solve the initial value problem.
$y''+2y'+2y=\left\{\begin{array}{rl}1,&0\le
t<2\pi,\\t,&2\pi\le t<3\pi,\\-1,&t\ge 3\pi,\end{array}\right.\;
y(0)=2,\quad y'(0)=-1$
\end{problem}

\begin{problem}\label{exer:8.5.21} Solve the initial value problem $$ y''=f(t), \quad
y(0)=0,\quad  y'(0)=0, $$ where $$ f(t)=m+1,\quad m\le t<m+1,\quad
m=0,1,2,\dots. $$
\end{problem}

\begin{problem}\label{exer:8.5.22} Solve the given initial value problem and find a
formula that does not involve step functions and represents $y$ on
each interval of continuity of $f$.
\begin{enumerate}
\item % (a)
$y''+y=f(t), \quad  y(0)=0,\quad  y'(0)=0$;

$f(t)=m+1,\quad  m\pi\le t<(m+1)\pi,\quad m=0,1,2,\dots$.

\item % (b)
$y''+y=f(t), \quad  y(0)=0,\quad y'(0)=0$;

$f(t)=(m+1)t, \quad   2m\pi\le t<2(m+1)\pi,\quad m=0,1,2,\dots$

\begin{hint}
You'll need the formula
$$
1+2+\cdots+m={m(m+1)\over2}.
$$  
\end{hint}

\item % (c)
$y''+y=f(t), \quad  y(0)=0,\quad  y'(0)=0$;

$f(t)=(-1)^m,\quad  m\pi\le t<(m+1)\pi,\quad m=0,1,2,\dots.$

\item % (d)
$y''-y=f(t), \quad  y(0)=0,\quad  y'(0)=0$;

$f(t)=m+1,\quad  m\le t<(m+1),\quad m=0,1,2,\dots.$

\begin{hint}
You will need the formula
$$
1+r+\cdots+r^m=\frac{1-r^{m+1}}{1-r}\; (r\ne1).
$$
\end{hint}

\item % (d)
$y''+2y'+2y=f(t), \quad  y(0)=0,\quad  y'(0)=0$;

$f(t)=(m+1)(\sin t+2\cos t),\quad  2m\pi\le t<2(m+1)\pi,\quad
m=0,1,2,\dots.$

\begin{hint}
You will need the formula
$$
1+r+\cdots+r^m=\frac{1-r^{m+1}}{1-r}\; (r\ne1).
$$
\end{hint}

\item % (f)
$y''-3y'+2y=f(t), \quad  y(0)=0,\quad y'(0)=0$;

$f(t)=m+1,\quad  m\le t<m+1,\quad m=0,1,2,\dots.$

\begin{hint}
You will need the formulas
$$
1+2+\cdots+m={m(m+1)\over2}.
$$ 
and
$$
1+r+\cdots+r^m=\frac{1-r^{m+1}}{1-r}\; (r\ne1).
$$
\end{hint}
\end{enumerate}
\end{problem}


\begin{problem}\label{exer:8.5.23}
\begin{enumerate}
\item % (a)
Let $g$ be  continuous on  $(\alpha,\beta)$
 and differentiable on the  $(\alpha,t_0)$
and $(t_0,\beta)$. Suppose $A=\lim_{t\to t_0-}g'(t)$
and $B=\lim_{t\to t_0+}g'(t)$ both exist. Use the mean value theorem
to show that
$$
\lim_{t\to t_0-}{g(t)-g(t_0)\over t-t_0}=A\quad\mbox{ and }\quad
\lim_{t\to t_0+}\frac{g(t)-g(t_0)}{t-t_0}=B.
$$
\item % (b)
Show we can conclude $g'(t_0)$ exists and $g'$ is continuous at
$t_0$ if $A=B$.

\item\label{exer:8.5.23c} % (c) 
Show we can also conclude
 that if $g$  is differentiable on $(\alpha,\beta)$ then
$g'$ cannot have a jump discontinuity on $(\alpha,\beta)$.
\end{enumerate}
\end{problem}

\begin{problem}\label{exer:8.5.24}
\begin{enumerate}
\item % (a)
Let $a$, $b$, and $c$ be constants, with $a\ne0$. Let $f$ be piecewise
continuous on an interval $(\alpha,\beta)$, with a single jump
discontinuity at a point $t_0$ in $(\alpha,\beta)$. Suppose $y$
and $y'$ are continuous on $(\alpha,\beta)$ and $y''$ on
$(\alpha,t_0)$ and $(t_0,\beta)$. Suppose  also that
$$
ay''+by'+cy=f(t) \quad
\text{(A)}
$$
on $(\alpha,t_0)$ and $(t_0,\beta)$.
Show that
$$
y''(t_0+)-y''(t_0-)={f(t_0+)-f(t_0-)\over a}\ne0.
$$
\item % (b)
Use the above exercise and Exercise~\ref{exer:8.5.23c} to show that
(A)
does not  have  solutions on any interval $(\alpha,\beta)$ that contains
a jump discontinuity of $f$.
\end{enumerate}
\end{problem}

\begin{problem}\label{exer:8.5.25}
Suppose $P_0,P_1$, and $P_2$ are continuous and $P_0$
has no zeros on an open interval $(a,b)$, and  that $F$
has a jump discontinuity at a point $t_0$ in $(a,b)$.
Show that the differential equation
$$
P_0(t)y''+P_1(t)y'+P_2(t)y=F(t)
$$
has no solutions on $(a,b)$.

\begin{hint}
Generalize the result of
Exercise~$\ref{exer:8.5.24}$ and use Exercise~$\ref{exer:8.5.23c}$.
\end{hint}
\end{problem}

\begin{problem}\label{exer:8.5.26}
Let $0=t_0<t_1<\cdots <t_n$. Suppose $f_m$ is continuous
on $[t_m,\infty)$ for $m=1,\dots,n$.
 Let
$$
f(t)=
\left\{\begin{array}{cl}
f_m(t),&t_m\le t< t_{m+1},\quad m=1,\dots,n-1,\\
f_n(t),&t\ge t_n.
\end{array}\right.
$$
Show that the
solution of
$$
ay''+by'+cy=f(t), \quad  y(0)=k_0,\quad y'(0)=k_1,
$$
as defined following  Theorem~\ref{thmtype:8.5.1}, is given by
$$
y=\left\{\begin{array}{cl}
 z_0(t),&0\le t<t_1,\\ 
z_0(t)+ z_1(t),&t_1\le t<t_2,\\
&\vdots\\
z_0+\cdots+z_{n-1}(t),&t_{n-1}\le t<t_n,\\ 
z_0+\cdots+ z_n(t),&t\ge t_n,
\end{array}\right.
$$
where $z_0$ is the solution of
$$
az''+bz'+cz=f_0(t), \quad  z(0)=k_0,\quad  z'(0)=k_1
$$
and $z_m$ is the solution of
$$
az''+bz'+cz=f_m(t)-f_{m-1}(t), \quad  z(t_m)=0,\quad z'(t_m)=0
$$
for $m=1,\dots,n$.
\end{problem}


\end{document}